examples/Baby.v
@@ -116,7 +116,7 @@ Definition always0 := bmodule "always0" {{
 (* Eval compute in compile always0. *)
 
 Theorem always0Ok : moduleOk always0.
-  vcgen; sep_auto.  
+  vcgen; sep_auto.
 Qed.
 
 (** Stress testing [structured] performance *)
